theories/g_stlc.v
@@ -1,5 +1,7 @@
 Require Export stlc.
 
+Import Lia.
+
 
 Module GStlc <: STLC.
   Declare Module Ty : TY.
@@ -81,6 +83,7 @@ Module GStlcTheories.
     (in custom stlc_tm at level 0, t custom stlc_tm) : stlc_scope.
   Notation "$( x )" := x
     (in custom stlc_tm at level 0, x constr, only parsing) : stlc_scope.
+  Notation "⊥" := gtm_bot (in custom stlc_tm) : stlc_scope.
   Notation "x \/ y" := (tm_app (tm_app gtm_or x) y)
     (in custom stlc_tm at level 60, left associativity) : stlc_scope.
   Notation "x /\ y" := (tm_app (tm_app gtm_and x) y)
@@ -96,24 +99,75 @@ Module GStlcTheories.
   Notation "'nab' T , t" := (tm_app (gtm_nab T) (tm_abs T t))
     (in custom stlc_tm at level 200, T custom stlc_ty,
       t custom stlc_tm at level 200, left associativity) : stlc_scope.
+  Notation "∇ T , t" := (tm_app (gtm_nab T) (tm_abs T t))
+    (in custom stlc_tm at level 200, T custom stlc_ty,
+      t custom stlc_tm at level 200, left associativity) : stlc_scope.
+  Notation "B ≡ C" := (<{(B > C) /\ (C > B)}>) (in custom stlc_tm at level 1) : stlc_scope.
+  Notation "~ B" := <{ B > gtm_bot }> (in custom stlc_tm at level 75) : stlc_scope.
 
+
+  (**************************************)
+  (** ** Nominal constants manipulation *)
+  (**************************************)
+
+  Fixpoint nom_prop (P : ty -> nat -> Prop) t : Prop :=
+    match t with
+    | gtm_nom T n => P T n
+    | gtm_app a b => nom_prop P a \/ nom_prop P b
+    | gtm_abs A a => nom_prop P a
+    | _ => False
+    end.
 
   Fixpoint nom_map (f : ty -> nat -> nat) t : tm :=
     match t with
     | gtm_nom T a => gtm_nom T (f T a)
-    | gtm_abs T t => tm_abs T (nom_map f t)
-    | gtm_app s t => tm_app (nom_map f s) (nom_map f t)
+    | gtm_abs T t => gtm_abs T (nom_map f t)
+    | gtm_app s t => gtm_app (nom_map f s) (nom_map f t)
     | x => x
     end.
 
-  Inductive invertible {A B} (f : A -> B) : Prop :=
-    invertible_intro g :
-      (forall x, f (g x) = x) ->
-      (forall x, g (f x) = x) ->
-      invertible f.
+  Instance pointwise2_Equiv A B C : Equiv (A -> B -> C) :=
+    fun f g => forall x y, f x y = g x y.
+
+  Theorem nom_map_Proper : Proper ((≡) ==> (=) ==> (=)) nom_map.
+  Proof.
+    intros f g E ? t ->. induction t; simpl; try easy; congruence.
+  Qed.
+
+  Theorem nom_map_comp f g t :
+    nom_map f (nom_map g t) = nom_map (fun T x => f T (g T x)) t.
+  Proof.
+    induction t; simpl; try easy; congruence.
+  Qed.
+
+  Theorem level_prop_nom_map P f t :
+    level_prop P (nom_map f t) <-> level_prop P t.
+  Proof.
+    induction t; simpl; try easy.
+    tm_simpl. intuition.
+  Qed.
+
+  Hint Rewrite level_prop_nom_map : tm.
+
+  (*
+  Theorem nom_map_app f s t :
+    nom_map f (tm_app s t) = tm_app (nom_map f s) (nom_map f t).
+  Proof. reflexivity. Qed.
+  *)
+
+  Theorem nom_map_id t : nom_map (fun _ => id) t = t.
+  Proof.
+    induction t; try easy; simpl; congruence.
+  Qed.
+
+  (*
+  Hint Rewrite nom_map_app nom_map_id : tm.
+  *)
+  Hint Rewrite nom_map_id : tm.
 
   Theorem has_type_nom_map f C T t :
-    has_type C t T <-> has_type C (nom_map f t) T.
+    has_type C (nom_map f t) T <->
+    has_type C t T.
   Proof.
     revert C T.
     induction t; intros C T; tm_simpl; try easy.
@@ -122,11 +176,202 @@ Module GStlcTheories.
     - split; intros H; inversion H; subst; now tm_simpl.
   Qed.
 
-  Inductive tm_equiv m : tm -> tm -> Prop :=
-    tm_equiv_intro a b f :
-      (forall T, invertible (f T)) -> lambda_equiv m a (nom_map f b) ->
-      tm_equiv m a b.
+  Theorem level_map_nom_map f g t :
+    level_map g (nom_map f t) = nom_map f (level_map g t).
+  Proof.
+    induction t; try easy; tm_simpl; now f_equal.
+  Qed.
 
+  (*
+  Theorem nom_map_lift f m t :
+    nom_map f (lift m t) = lift m (nom_map f t).
+  Proof.
+    induction t; try easy.
+    - unfold lift, bound_level_map in *. rewrite level_map_app.
+      rewrite nom_map_app. rewrite IHt1, IHt2. now tm_simpl.
+    - unfold lift, bound_level_map in *. rewrite level_map_abs.
+      tm_simpl. now rewrite IHt.
+  Qed.
+  *)
+
+  Theorem nom_map_subst f m l t :
+    nom_map f (subst m l t) = subst m (nom_map f <$> l) (nom_map f t).
+  Proof.
+    revert m l.
+    induction t; intros m l; try easy; tm_simpl.
+    - unfold lookup_default. simpl. destruct (decide (n < l)).
+      + now rewrite decide_True.
+      + now rewrite decide_False.
+    - now f_equal.
+    - rewrite IHt. f_equal. apply subst_Proper; [|reflexivity].
+      constructor; [reflexivity|].
+      intros n Hn. simpl in *. destruct (decide (n < l)).
+      + rewrite decide_True; [|easy]. symmetry. apply level_map_nom_map.
+      + rewrite decide_False; easy.
+  Qed.
+
+  Theorem nom_map_subst_last f n m s t :
+    nom_map f (subst_last n m s t) = subst_last n m (nom_map f s) (nom_map f t).
+  Proof.
+    unfold subst_last. rewrite nom_map_subst.
+    apply subst_Proper; [|reflexivity].
+    simpl. constructor; [reflexivity|].
+    intros a Ha. simpl in *. now destruct (decide (a < n)).
+  Qed.
+
+  Hint Rewrite nom_map_subst_last : tm.
+
+  Theorem lambda_equiv_nom_map m a b f :
+    lambda_equiv m a b -> lambda_equiv m (nom_map f a) (nom_map f b).
+  Proof.
+    intros H.
+    eapply rtsc_congruence; [|eassumption]. clear H.
+    intros x y H.
+    induction H; subst.
+    - constructor. destruct H; destruct H; simpl.
+      + left. rewrite nom_map_subst_last. constructor.
+      + right. unfold bound_level_map. rewrite <- level_map_nom_map.
+        constructor. unfold contains_bound_levels. now tm_simpl.
+    - tm_simpl. now apply step_appL.
+    - tm_simpl. now apply step_appR.
+    - tm_simpl. now apply step_abs.
+  Qed.
+
+
+  (** *** Support *)
+
+  Definition in_supp t n := nom_prop (fun T x => n = gtm_nom T x) t.
+
+  Theorem in_supp_other t n : in_supp t n -> tm_other n.
+  Proof.
+    intros H. unfold in_supp in H.
+    induction t; try easy; tm_simpl in H; intuition.
+    now subst.
+  Qed.
+
+  Fixpoint nom_fresh t : nat :=
+    match t with
+    | gtm_nom _ n => S n
+    | gtm_app a b => max (nom_fresh a) (nom_fresh b)
+    | gtm_abs A a => nom_fresh a
+    | _ => 0
+    end.
+
+  Theorem nom_fresh_le_in_supp t T :
+    forall n, nom_fresh t <= n -> ~ in_supp t (gtm_nom T n).
+  Proof.
+    intros n Hn N.
+    induction t; unfold in_supp in *; simpl in *; try easy.
+    - destruct N.
+      + apply IHt1; [lia|assumption].
+      + apply IHt2; [lia|assumption].
+    - auto.
+    - injection N. lia.
+  Qed.
+
+  Theorem nom_fresh_in_supp t T : ~ in_supp t (gtm_nom T (nom_fresh t)).
+  Proof. now apply nom_fresh_le_in_supp. Qed.
+
+
+  (************************)
+  (** ** Term equivalence *)
+  (************************)
+
+  Inductive tm_equiv m a b : Prop :=
+    tm_equiv_intro f g :
+      (forall T x, g T (f T x) = x) -> (forall T x, f T (g T x) = x) ->
+      lambda_equiv m a (nom_map f b) ->
+      tm_equiv m a b.
+  Arguments tm_equiv_intro {m a b}.
+
+  Instance tm_equiv_equivalence m : Equivalence (tm_equiv m).
+  Proof.
+    constructor; intros a.
+    - eapply (tm_equiv_intro (fun _ x => x)); try reflexivity.
+      now tm_simpl.
+    - intros b [f g Hgf Hfg]. econstructor.
+      + apply Hfg.
+      + apply Hgf.
+      + symmetry.
+        replace b with (nom_map g (nom_map f b)); [now apply lambda_equiv_nom_map|].
+        rewrite <- (nom_map_id b) at 2.
+        rewrite nom_map_comp. now apply nom_map_Proper.
+    - intros y z [f g Hgf Hfg] [h l Hlh Hhl].
+      eapply (tm_equiv_intro (fun T x => f T (h T x)) (fun T x => l T (g T x)));
+        try congruence.
+      etransitivity; [eassumption|].
+      rewrite <- (nom_map_comp f h).
+      now apply lambda_equiv_nom_map.
+  Qed.
+
+  (*
+  Definition nom_swap (T : ty) (n m : nat) A a :=
+    if (decide (A = T)) then (
+      if (decide (a = n)) then m else (
+        if (decide (a = m)) then n else a
+      )
+    ) else a.
+
+  Theorem nom_swap_eq T n m : nom_swap T n m T n = m.
+  Proof.
+    unfold nom_swap. now repeat rewrite decide_True.
+  Qed.
+
+  Theorem nom_swap_neq T n m A x :
+    x <> n -> x <> m -> nom_swap T n m A x = x.
+  Proof.
+    intros. unfold nom_swap. destruct (decide (A = T)); [|reflexivity].
+    now repeat rewrite decide_False.
+  Qed.
+
+  Hint Rewrite nom_swap_eq : tm.
+
+  Theorem in_supp_nom_map f t :
+    (forall T n, in_supp t (gtm_nom T n) -> f T n = n) ->
+    nom_map f t = t.
+  Proof.
+    intros H. induction t; simpl in *; try reflexivity.
+    - rewrite IHt1, IHt2; try reflexivity.
+      + intros. apply H. unfold in_supp in *. simpl. intuition.
+      + intros. apply H. unfold in_supp in *. simpl. intuition.
+    - rewrite IHt; [reflexivity|].
+      intros. auto.
+    - f_equal. now apply H.
+  Qed.
+
+  Theorem in_supp_nom_swap T m n t :
+    ~ in_supp t (gtm_nom T n) -> ~ in_supp t (gtm_nom T m) ->
+    nom_map (nom_swap T m n) t = t.
+  Proof.
+    intros. apply in_supp_nom_map. intros.
+    destruct (decide (T = T0)).
+    - subst. apply nom_swap_neq; intros N; subst; contradiction.
+    - unfold nom_swap. now rewrite decide_False.
+  Qed.
+
+  Theorem nom_swap_tm_equiv m T x y a b :
+    lambda_equiv m a (nom_map (nom_swap T x y) b) -> tm_equiv m a b.
+  Proof.
+    intros LE.
+    apply (tm_equiv_intro (nom_swap T x y) (nom_swap T y x)); try assumption.
+    - intros X t. unfold nom_swap.
+      destruct (decide (X = T)); [|reflexivity].
+      destruct (decide (t = x)), (decide (t = y)), (decide (x = y)); subst;
+        try (now rewrite decide_True).
+      + reflexivity.
+      + now repeat rewrite decide_False.
+      + now repeat rewrite decide_False.
+    - intros X t. unfold nom_swap.
+      destruct (decide (X = T)); [|reflexivity].
+      destruct (decide (t = x)), (decide (t = y)), (decide (y = x)); subst;
+        try (now rewrite decide_True).
+      + reflexivity.
+      + now repeat rewrite decide_False.
+      + now repeat rewrite decide_False.
+  Qed.
+  *)
+
+  (*
   Theorem has_type_tm_equiv (C : context) T a b : tm_equiv C a b ->
     has_type C a T -> has_type C b T.
   Proof.
@@ -134,15 +379,18 @@ Module GStlcTheories.
     eapply has_type_nom_map.
     eapply has_type_lambda_equiv; eassumption.
   Qed.
+  *)
 
-  Inductive in_supp : tm -> tm -> Prop :=
-    | is_nom T n : in_supp (gtm_nom T n) (gtm_nom T n)
-    | is_appL a b n : in_supp a n -> in_supp (gtm_app a b) n
-    | is_appR a b n : in_supp b n -> in_supp (gtm_app a b) n
-    | is_abs T t n : in_supp t n -> in_supp (gtm_abs T t) n.
 
-  Theorem in_supp_other b t : in_supp b t -> tm_other t.
-  Proof. intros H. induction H; easy. Qed.
+  (*
+  Theorem subst_gtm_bot n l : subst n l gtm_bot = gtm_bot.
+  Proof. now tm_simpl. Qed.
+
+  Theorem subst_last_gtm_bot m n s : subst_last m n s gtm_bot = gtm_bot.
+  Proof. now tm_simpl. Qed.
+
+  Hint Rewrite subst_gtm_bot subst_last_gtm_bot : tm.
+  *)
 End GStlcTheories.
 
 
