theories/rlist.v
@@ -9,6 +9,7 @@ Record rlist (A : Type) : Type := {
 Arguments Build_rlist {A}.
 Arguments rl_length {A}.
 Arguments rl_map {A}.
+Add Printing Constructor rlist.
 
 Declare Scope rlist_scope.
 Delimit Scope rlist_scope with rlist.
@@ -26,117 +27,42 @@ Notation "l +: e" := (rl_cons l e) (at level 50) : rlist_scope.
 Instance rlist_fmap : FMap rlist :=
   fun _ _ f l => Build_rlist l (fun n => f (l n)).
 
-(*
-Theorem rlength_rcons : forall {A} (c : rlist A) t,
-  rlength (rcons c t) = S (rlength c).
+
+Instance rlist_empty {A} `{Inhabited A} : Empty (rlist A) :=
+  Build_rlist 0 inhabitant.
+
+Inductive rlist_equiv {A} (l : rlist A) m : Prop :=
+  rlist_equiv_intro : rl_length l = rl_length m ->
+    (forall n, n < l -> l n = m n) ->
+    rlist_equiv l m.
+
+Instance rlist_Equiv {A} : Equiv (rlist A) := rlist_equiv.
+
+Instance rlist_equiv_Equivalence A : Equivalence (@rlist_equiv A).
 Proof.
-  intros. unfold rcons. apply rlength_build_rlist.
+  constructor; intros x.
+  - now constructor.
+  - intros y H. destruct H.
+    constructor; [easy|].
+    intros. symmetry. apply H0. congruence.
+  - intros y z Hx Hz. destruct Hx, Hz.
+    constructor; [congruence|].
+    intros. rewrite H0; [rewrite H2|]; congruence.
 Qed.
 
-Theorem lookup_rcons_eq : forall {A} (c : rlist A) t n,
-  n = rlength c -> rcons c t !! n = Some t.
+Instance rl_length_Proper {A} : Proper ((≡) ==> (=)) (@rl_length A).
+Proof. intros x y E. now destruct E. Qed.
+
+Instance rlist_fmap_Proper {A B} : Proper ((=) ==> (≡) ==> (≡)) (rlist_fmap A B).
 Proof.
-  intros.
-  unfold rcons. rewrite lookup_build_rlist; [|lia].
-  f_equal. rewrite decide_False; [easy|lia].
+  intros ? f -> x y E. destruct E. constructor.
+  - now simpl.
+  - intros. simpl in *. now rewrite H0.
 Qed.
 
-Theorem lookup_rcons_lt : forall {A} (c : rlist A) t n,
-  n < rlength c -> (c +: t) !! n = c !! n.
+Instance rl_cons_Proper {A} : Proper ((≡) ==> (=) ==> (≡)) (@rl_cons A).
 Proof.
-  intros * H.
-  unfold rcons. rewrite lookup_build_rlist; [|lia].
-  apply is_Some_lookup in H as Hx. destruct Hx as [x Hx]. rewrite Hx.
-  f_equal. rewrite decide_True; [|easy].
-  unfold lookup_default. now rewrite Hx.
+  intros x y E ? a ->. destruct E. constructor.
+  - simpl. congruence.
+  - intros. simpl in *. rewrite H in *. destruct (decide (n < y)); auto.
 Qed.
-
-Theorem lookup_rcons_gt : forall {A} (c : rlist A) t n,
-  n > |(c)| -> rcons c t !! n = None.
-Proof.
-  intros. apply lookup_None1.
-  rewrite rlength_rcons. lia.
-Qed.
-
-Inductive lookup_rcons_cases {A} (c : rlist A) t n : Prop :=
-  | lookup_rcons_cases_lt (_ : n < |(c)|) (_ : (c +: t) !! n = c !! n)
-  | lookup_rcons_cases_eq (_ : n = |(c)|) (_ : (c +: t) !! n = Some t)
-  | lookup_rcons_cases_gt (_ : n > |(c)|) (_ : (c +: t) !! n = None).
-
-Theorem lookup_rcons_spec {A} (c : rlist A) t n : lookup_rcons_cases c t n.
-Proof.
-  destruct (lt_total n |(c)|) as [H | [H | H]].
-  - apply lookup_rcons_cases_lt; [assumption|].
-    now apply lookup_rcons_lt.
-  - apply lookup_rcons_cases_eq; [assumption|].
-    now apply lookup_rcons_eq.
-  - apply lookup_rcons_cases_gt; [assumption|].
-    now apply lookup_rcons_gt.
-Qed.
-
-Ltac lookup_rcons_spec c t n H E :=
-  destruct (lookup_rcons_spec c t n) as [H E | H E | H E]; rewrite E in *.
-
-Theorem is_Some_rlength {A B} (l : rlist A) (h : rlist B) :
-  (forall n, is_Some (l !! n) <-> is_Some (h !! n)) ->
-  |(l)| = |(h)|.
-Proof.
-  intros H. destruct (lt_total |(l)| |(h)|) as [E|[L|G]]; try assumption.
-  - apply is_Some_lookup in E. apply H in E.
-    apply is_Some_lookup in E. lia.
-  - apply is_Some_lookup in G. apply H in G.
-    apply is_Some_lookup in G. lia.
-Qed.
-
-Theorem rlength_fmap : forall {A} {B} (f : A -> B) l,
-  |(f <$> l)| = |(l)|.
-Proof.
-  intros. apply is_Some_rlength.
-  intros. rewrite lookup_fmap. apply fmap_is_Some.
-Qed.
-End RlistTheories.
-
-
-(** ** Reverse list implementation *)
-
-Module RlistList <: RLIST.
-Definition rlist := list.
-Definition rlength := @length.
-
-Instance rlist_lookup {A} : Lookup nat A (rlist A) := list_lookup.
-
-Theorem is_Some_lookup {A} :
-  forall (c : rlist A) n, is_Some (c !! n) <-> n < length c.
-Proof. apply lookup_lt_is_Some. Qed.
-
-Fixpoint build_rlist {A} n f : rlist A :=
-  match n with
-  | 0 => []
-  | S n => build_rlist n f ++ [f n]
-  end.
-
-Theorem rlength_build_rlist : forall {A} n (f : nat -> A),
-  length (build_rlist n f) = n.
-Proof.
-  intros. induction n; [reflexivity|].
-  simpl. rewrite length_app. rewrite IHn. simpl. lia.
-Qed.
-
-Theorem lookup_build_rlist : forall {A} n (f : nat -> A) x,
-  x < n -> build_rlist n f !! x = Some (f x).
-Proof.
-  intros. induction n; [lia|].
-  simpl. destruct (decide (x = n)).
-  - subst. rewrite @lookup_app_r; rewrite rlength_build_rlist; [|lia].
-    now rewrite sub_diag.
-  - rewrite @lookup_app_l.
-    + apply IHn. lia.
-    + rewrite rlength_build_rlist. lia.
-Qed.
-
-Instance rlist_fmap : FMap rlist := list_fmap.
-
-Theorem lookup_fmap : forall {A} {B} (f : A -> B) (l : rlist A) n,
-  (f <$> l) !! n = f <$> l !! n.
-Proof. intros. apply list_lookup_fmap. Qed.
-*)
